wip: lambda example

hs-to-coq/examples/lambda/Proofs.v
@@ -19,11 +19,14 @@ end.
 Fixpoint depth e := match e with 
   | Mk_Var v' => 0
   | Mk_Lam v' e => S (depth e)
-  | Mk_App e1 e2 => PeanoNat.Nat.max (S (depth e1)) (S (depth e2))
-  | Mk_Let v' rhs body =>  PeanoNat.Nat.max (S (depth rhs)) (S (depth body))
+  | Mk_App e1 e2 =>
+    PeanoNat.Nat.max (S (depth e1)) (S (depth e2))
+  | Mk_Let v' rhs body =>
+    PeanoNat.Nat.max (S (depth rhs)) (S (depth body))
 end.
 
-Lemma depth_rename : forall v w e, depth (rename v w e) = depth e.
+Lemma depth_rename : forall v w e,
+    depth (rename v w e) = depth e.
 Proof.
   intros.
   induction e.
@@ -44,27 +47,200 @@ Qed.
 Require Import Recdef.
 
 
-Function subst v arg body {measure depth body} := match body with
+Function subst v arg body {measure depth body} :=
+  match body with
   | Mk_Var v' => if v == v' then arg else Mk_Var v'
   | Mk_Lam v' e => if v == v' then Mk_Lam v' e else
-    let f := fresh e in
-    Mk_Lam f (subst v arg (rename v' v e))
+                    let f := fresh e in
+                    Mk_Lam f (subst v arg (rename v' v e))
   | Mk_App e1 e2 => Mk_App (subst v arg e1)  (subst v arg e2)
   | Mk_Let v' rhs body =>
     let v'' := fresh body in
     let rhs' := subst v arg rhs in
     let body' := subst v arg (rename v' v'' body) in
     Mk_Let v' rhs' body'
-end.
+  end.
 Proof.
- all: intros; simpl; repeat rewrite depth_rename; zify; omega.
+  all: intros; simpl;
+    repeat rewrite depth_rename; zify; omega.
 Qed.
 
-Inductive ss : Expr -> Expr -> Prop :=
-  | ss_beta : forall v body arg, isVal arg -> ss (Mk_App (Mk_Lam v body) arg) (subst v arg body)
-  | ss_let: forall v body rhs , isVal rhs -> ss (Mk_Let v rhs body) (subst v rhs body)
-  | ss_let_search: forall v body rhs rhs', ss rhs rhs' -> ss (Mk_Let v rhs body) (Mk_Let v rhs' body)
-  | ss_app_search : forall m m' n, ss m m' -> ss (Mk_App m n) (Mk_App m' n)
-  | ss_app_val: forall m n n', isVal m -> ss n n' -> ss (Mk_App m n) (Mk_App m n')
-.
+Inductive small_step : Expr -> Expr -> Prop :=
+| ss_beta : forall v body arg,
+    isVal arg ->
+    small_step (Mk_App (Mk_Lam v body) arg) (subst v arg body)
+| ss_let: forall v body rhs ,
+    isVal rhs ->
+    small_step (Mk_Let v rhs body) (subst v rhs body)
+| ss_let_search: forall v body rhs rhs',
+    small_step rhs rhs' ->
+    small_step (Mk_Let v rhs body) (Mk_Let v rhs' body)
+| ss_app_search : forall m m' n,
+    small_step m m' ->
+    small_step (Mk_App m n) (Mk_App m' n)
+| ss_app_val: forall m n n',
+    isVal m ->
+    small_step n n' ->
+    small_step (Mk_App m n) (Mk_App m n').
 
+
+Fixpoint small_step_fun (t : Expr) : option Expr :=
+  match t with
+  | Mk_App t1 t2 => match t1 with
+                | Mk_Lam v t3 =>
+                  match small_step_fun t2 with
+                  | Some t2' => Some (Mk_App t1 t2')
+                  | _ => match t2 with
+                        | Mk_App _ _ => None
+                        | _ => Some (subst v t2 t3)
+                        end
+                  end
+                | Mk_Var i =>
+                  match small_step_fun t2 with
+                    | Some t2' => Some (Mk_App t1 t2')
+                    | _ => None
+                    end
+                | _ => match (small_step_fun t1) with
+                      | Some t1' => Some (Mk_App t1' t2)
+                      | _ => None
+                      end
+                   end
+  | Mk_Let v t1 t2 =>
+    match t1 with
+      | Mk_Var _ => Some (subst v t1 t2)
+      | Mk_Lam _ _ => Some (subst v t1 t2)
+      | _ => match (small_step_fun t1) with
+            | Some t1' => Some (Mk_Let v t1' t2)
+            | _ => None
+            end
+    end
+  | _ => None
+  end.
+
+Lemma isVal_not_step: forall n,
+    isVal n -> small_step_fun n = None.
+Proof.
+  intros []; auto;
+  intros H; inversion H.
+Qed.  
+
+
+Lemma small_step_small_step_fun : forall m m',
+  small_step m m' <-> small_step_fun m = Some m'.
+Proof.
+  split.
+  - induction 1.
+    + simpl. rewrite isVal_not_step; auto.
+      destruct arg; auto. inversion H.
+    + simpl.
+      destruct rhs; auto;
+        inversion H; subst.
+    + inversion H; subst.
+      * simpl in IHsmall_step.
+        simpl.
+        destruct (small_step_fun arg).
+        -- inversion IHsmall_step; auto.
+        -- destruct arg; auto. inversion IHsmall_step.
+      * simpl in IHsmall_step.
+        simpl.
+        destruct rhs0; auto.
+        -- destruct (small_step_fun (Mk_Let n rhs0_1 rhs0_2)).
+           inversion IHsmall_step. auto.
+        -- inversion IHsmall_step.
+      * destruct (small_step_fun (Mk_App rhs0_1 rhs0_2));
+          inversion IHsmall_step; auto.
+      * simpl in IHsmall_step.
+        simpl.        
+        destruct rhs0.
+        -- inversion IHsmall_step. auto.
+        -- destruct (small_step_fun (Mk_Let n rhs0_1 rhs0_2)).
+           inversion IHsmall_step. auto.
+        -- inversion IHsmall_step.
+        -- inversion IHsmall_step. auto.
+        -- destruct (small_step_fun (Mk_App rhs0_1 rhs0_2));
+             inversion IHsmall_step; auto.
+        - simpl in IHsmall_step.
+           simpl.
+           destruct m; try solve [inversion H0].
+           ++ destruct (small_step_fun (Mk_Let n0 m1 m2));
+                inversion IHsmall_step; subst; auto.
+           ++ destruct (small_step_fun (Mk_App m1 m2));
+                inversion IHsmall_step; auto.
+        -- simpl in IHsmall_step.
+           simpl.
+           destruct m; try solve [inversion H0].
+           ++ destruct (small_step_fun n);
+                inversion IHsmall_step; subst; auto.
+           ++ destruct (small_step_fun n);
+                inversion IHsmall_step; subst; auto.
+              destruct n;
+                try solve [inversion H1| inversion H3].
+              inversion H3. auto.
+        -- destruct m;
+             try solve [inversion IHsmall_step];
+                 simpl in IHsmall_step;
+                 simpl.
+           ++ destruct m1; inversion IHsmall_step; auto.
+              ** destruct (small_step_fun
+                             (Mk_Let n1 m1_1 m1_2));
+                   inversion IHsmall_step; auto.
+              ** destruct (small_step_fun
+                             (Mk_App m1_1 m1_2));
+                   inversion IHsmall_step; auto.
+        + simpl. simpl in IHsmall_step.
+              intuition.
+              ** inversion IHsmall_step. subst. auto.
+              **  admit.
+                  admit.
+                  admit.
+Admitted.
+
+
+Inductive rtc {A} (R:A -> A -> Prop) : A -> A -> Prop :=
+| rtc_refl : forall a, rtc R a a
+| rtc_step : forall a b c, R a b -> rtc R b c -> rtc R a c.
+
+Notation "R ^*" := (rtc R) (at level 1, format "R ^*").
+
+Definition nf (x: Expr): Prop := ~ exists y, small_step x y.
+
+Inductive beta_equiv : Expr -> Expr -> Prop :=
+| be_refl: forall x, beta_equiv x y
+| be_
+| be_Step: forall v x y,
+    beta_equiv (Mk_Let v x y) (Mk_App (Mk_Lam v y) x)
+               
+| be_Var : forall v, beta_equiv (Mk_Var v) (Mk_Var v)
+| be_Let: forall v x1 x2 y1 y2,
+    beta_equiv x1 x2 -> beta_equiv y1 y2 ->
+    beta_equiv (Mk_Let v x1 y1) (Mk_Let v x2 y2)
+| be_App: forall x1 x2 y1 y2,
+    beta_equiv x1 x2 -> beta_equiv y1 y2 ->
+    beta_equiv (Mk_App x1 y1) (Mk_App x2 y2)
+| be_Lam: forall v x1 x2,
+    beta_equiv x1 x2 ->
+    beta_equiv (Mk_Lam v x1) (Mk_Lam v x2).
+                           
+| ss_beta : forall v body arg,
+    isVal arg ->
+    small_step (Mk_App (Mk_Lam v body) arg) (subst v arg body)
+| ss_let: forall v body rhs ,
+    isVal rhs ->
+    small_step (Mk_Let v rhs body) (subst v rhs body)
+
+(* 
+Let x y z ==  App (Lam x z)  y
+
+
+
+    Lam x (App x (Lam y y)) is nf
+anf (Lam x (App x (Lam y y))) = 
+     Lam x (Let z = (Lam y y) in x z)
+*)
+Theorem anf_correct: forall x y,
+    small_step^* x y -> nf y ->
+    small_step^* (anf x) y' /\ R y y'.
+Proof.
+  intros x y Hs Hn.
+  
+  
